Began cotree lore

Gt3/Syntax/Tree/Defs/Tree.lean
@@ -1,23 +1,8 @@
-import Gt3.Syntax.Tree.Defs.Index
-import Gt3.Syntax.Tree.Children
+import Gt3.Syntax.Tree.Defs.Node
 
 namespace Gt3
 
 open NumChildren BinderList HasChildren CastLE
-
-/-- A single node -/
-structure Node (α : Type _) [NumChildren α] (β : Type _) : Type _ where
-  tag : α
-  children : Fin (numChildren tag) → β
-
-instance {α} [NumChildren α] {β} : NumChildren (Node α β) where
-  numChildren n := numChildren n.tag
-
-instance {α} [BinderList α] {β} : BinderList (Node α β) where
-  binderList n := binderList n.tag
-
-instance {α} [BinderList α] {β} : FlatChildren (Node α β) β where
-  getChild n := n.children
 
 /-- A tree of nodes -/
 structure Tree (α : Type _) [NumChildren α] : Type _ where
@@ -36,7 +21,7 @@ instance {α} [BinderList α] : BinderList (Tree α) where
   binderList t := binderList t.tag
 
 instance {α} [BinderList α] : FlatChildren (Tree α) (Tree α) where
-  getChild t := t.children
+  getDChild t := t.children
 
 def Node.toTree {α} [NumChildren α] (n : Node α (Tree α)) : Tree α :=
   ⟨n.tag, n.children⟩
@@ -68,25 +53,6 @@ theorem Tree.toNode_toTree {α} [NumChildren α] (t : Tree α) : t.toNode.toTree
 theorem Node.toTree_toNode {α} [NumChildren α] (n : Node α (Tree α)) : n.toTree.toNode = n
   := by cases n; rfl
 
-def Node.map {α α' β β'} [NumChildren α] [NumChildren α']
-  (f : α → α') [hf : NumChildrenHom f]
-  (g : β → β') (n : Node α β) : Node α' β' :=
-  ⟨f n.tag, fun i => g (n.children (i.cast (hf.numChildren_hom n.tag)))⟩
-
-def Node.mapTag {α α' β} [NumChildren α] [NumChildren α']
-  (f : α → α') [hf : NumChildrenHom f] (n : Node α β) : Node α' β := n.map f id
-
-def Node.mapChildren {α β β'} [NumChildren α] (f : β → β') (n : Node α β) : Node α β' :=
-  ⟨n.tag, fun i => f (n.children i)⟩
-
-instance Node.instFunctor {α} [NumChildren α] : Functor (Node α) where
-  map := Node.mapChildren
-
-instance Node.instLawfulFunctor {α} [NumChildren α] : LawfulFunctor (Node α) where
-  map_const := rfl
-  id_map _ := rfl
-  comp_map _ _ _ := rfl
-
 def Node.mapToTree {α α' β} [NumChildren α] [NumChildren α']
   (f : α → α') [hf : NumChildrenHom f]
   (g : β → Tree α')
@@ -95,20 +61,6 @@ def Node.mapToTree {α α' β} [NumChildren α] [NumChildren α']
 
 def Node.treeChildren {α β} [NumChildren α] (n : Node α β) (f : β → Tree α) : Tree α :=
   ⟨n.tag, fun i => f (n.children i)⟩
-
-instance Node.map_numChildrenHom {α α' β β'} [NumChildren α] [NumChildren α']
-  (f : α → α') [hf : NumChildrenHom f] (g : β → β')
-  : NumChildrenHom (Node.map f g) where
-  numChildren_hom _ := hf.numChildren_hom _
-
-instance Node.mapTag_numChildrenHom {α α' β} [NumChildren α] [NumChildren α']
-  (f : α → α') [hf : NumChildrenHom f]
-  : NumChildrenHom (Node.mapTag (β := β) f) where
-  numChildren_hom _ := hf.numChildren_hom _
-
-instance Node.mapChildren_numChildrenHom {α β β'} [NumChildren α]
-  (f : β → β') : NumChildrenHom (Functor.map (f := Node α) f) where
-  numChildren_hom _ := rfl
 
 -- instance Node.instCastLE {ι} [PartialOrder ι] {α}
 --   [∀ n, BinderList (α n)] {β} [BindCastLE α] [CastLE β]
