Gt3/Syntax/Tree/Children.lean
@@ -6,11 +6,13 @@ open NumChildren BinderList
 
 /-- A node equipped with a set of children of indexed type `β` -/
 class HasChildren (α : Type _) [BinderList α] (β : ℕ → Type _) where
-  getChild (t : α) : (i : Fin (numChildren t)) → (β (getBinder t i))
+  getDChild (t : α) : (i : Fin (numChildren t)) → (β (getBinder t i))
 
 open HasChildren
 
 class FlatChildren (α : Type _) [BinderList α] (β : Type _) extends HasChildren α (fun _ => β) where
+  getChild (t : α) : (i : Fin (numChildren t)) → β := getDChild t
+  getChild_eq (t : α) (i : Fin (numChildren t)) : getChild t i = getDChild t i := by intros; rfl
   listChildren (t : α) : List β := List.ofFn (getChild t)
   listChildren_eq (t : α) : listChildren t = List.ofFn (getChild t) := by simp
 
