Gt3/Syntax/Tree/Defs/Node.lean
@@ -1,0 +1,57 @@
+import Gt3.Syntax.Tree.Defs.Index
+import Gt3.Syntax.Tree.Children
+
+namespace Gt3
+
+open NumChildren BinderList HasChildren CastLE
+
+/-- A single node -/
+structure Node (α : Type _) [NumChildren α] (β : Type _) : Type _ where
+  tag : α
+  children : Fin (numChildren tag) → β
+
+instance Node.instNumChildren {α} [NumChildren α] {β} : NumChildren (Node α β) where
+  numChildren n := numChildren n.tag
+
+instance Node.instBinderList {α} [BinderList α] {β} : BinderList (Node α β) where
+  binderList n := binderList n.tag
+
+instance Node.instHasChildren {α} [BinderList α] {β} : HasChildren (Node α β) (fun _ => β) where
+  getDChild n := n.children
+
+instance Node.instFlatChildren {α} [BinderList α] {β} : FlatChildren (Node α β) β where
+
+def Node.map {α α' β β'} [NumChildren α] [NumChildren α']
+  (f : α → α') [hf : NumChildrenHom f]
+  (g : β → β') (n : Node α β) : Node α' β' :=
+  ⟨f n.tag, fun i => g (n.children (i.cast (hf.numChildren_hom n.tag)))⟩
+
+def Node.mapTag {α α' β} [NumChildren α] [NumChildren α']
+  (f : α → α') [hf : NumChildrenHom f] (n : Node α β) : Node α' β := n.map f id
+
+def Node.mapChildren {α β β'} [NumChildren α] (f : β → β') (n : Node α β) : Node α β' :=
+  ⟨n.tag, fun i => f (n.children i)⟩
+
+instance Node.instFunctor {α} [NumChildren α] : Functor (Node α) where
+  map := Node.mapChildren
+
+instance Node.instLawfulFunctor {α} [NumChildren α] : LawfulFunctor (Node α) where
+  map_const := rfl
+  id_map _ := rfl
+  comp_map _ _ _ := rfl
+
+instance Node.map_numChildrenHom {α α' β β'} [NumChildren α] [NumChildren α']
+  (f : α → α') [hf : NumChildrenHom f] (g : β → β')
+  : NumChildrenHom (Node.map f g) where
+  numChildren_hom _ := hf.numChildren_hom _
+
+instance Node.mapTag_numChildrenHom {α α' β} [NumChildren α] [NumChildren α']
+  (f : α → α') [hf : NumChildrenHom f]
+  : NumChildrenHom (Node.mapTag (β := β) f) where
+  numChildren_hom _ := hf.numChildren_hom _
+
+instance Node.mapChildren_numChildrenHom {α β β'} [NumChildren α]
+  (f : β → β') : NumChildrenHom (Functor.map (f := Node α) f) where
+  numChildren_hom _ := rfl
+
+end Gt3
